code/experimental/gf128/Hacl.Gf128.PreComp.fst
@@ -2,88 +2,94 @@ module Hacl.Gf128.PreComp
 
 open FStar.HyperStack
 open FStar.HyperStack.All
+
 open Lib.IntTypes
 open Lib.Buffer
+open Lib.IntVector
+
 open Hacl.Impl.Gf128.Fields
 open Hacl.Impl.Gf128.Generic
 
 module ST = FStar.HyperStack.ST
 
+module S = Spec.GF128
+module GF = Spec.GaloisField
+module Vec = Hacl.Spec.GF128.Vec
 
+
+#reset-options "--z3rlimit 50 --max_fuel 0 --max_ifuel 1"
+
+inline_for_extraction noextract
 let gcm_ctx_elem = uint64
+inline_for_extraction noextract
 let gcm_ctx_len = 266ul
+inline_for_extraction noextract
 let gcm_ctx_elem_zero = u64 0
+inline_for_extraction noextract
 let gcm_ctx = lbuffer gcm_ctx_elem gcm_ctx_len
 
 
-[@ CInline ]
+[@CInline]
 val gcm_init:
-    ctx: gcm_ctx
-  -> key: lbuffer uint8 16ul ->
+    ctx:gcm_ctx
+  -> key:lbuffer uint8 16ul ->
   Stack unit
-  (requires (fun h -> live h ctx /\ live h key))
-  (ensures (fun h0 _ h1 -> modifies1 ctx h0 h1))
+  (requires fun h -> live h ctx /\ live h key /\ disjoint ctx key)
+  (ensures  fun h0 _ h1 -> modifies1 ctx h0 h1)
 
-let gcm_init ctx key = gcm_init #F32 ctx key
+let gcm_init ctx key = gcm_init #Vec.PreComp ctx key
 
 
-inline_for_extraction
+[@CInline]
 val gcm_update_blocks:
-    ctx: gcm_ctx
-  -> len: size_t
-  -> text: lbuffer uint8 len ->
+    ctx:gcm_ctx
+  -> len:size_t
+  -> text:lbuffer uint8 len ->
   Stack unit
-  (requires (fun h -> live h ctx /\ live h text))
-  (ensures (fun h0 _ h1 -> modifies1 ctx h0 h1))
+  (requires fun h -> live h ctx /\ live h text)
+  (ensures  fun h0 _ h1 -> modifies1 ctx h0 h1)
 
-let gcm_update_blocks  ctx len text = poly4_mul_add #F32 ctx len text
+let gcm_update_blocks ctx len text =
+  let acc = get_acc ctx in
+  let pre = get_precomp ctx in
+  gf128_update_vec #Vec.PreComp acc pre len text
 
 
-inline_for_extraction
+[@CInline]
 val gcm_update_blocks_padded:
-    ctx: gcm_ctx
-  -> len: size_t
-  -> text: lbuffer uint8 len ->
+    ctx:gcm_ctx
+  -> len:size_t
+  -> text:lbuffer uint8 len ->
   Stack unit
-  (requires (fun h -> live h ctx /\ live h text))
-  (ensures (fun h0 _ h1 -> modifies1 ctx h0 h1))
+  (requires fun h -> live h ctx /\ live h text)
+  (ensures  fun h0 _ h1 -> modifies1 ctx h0 h1)
 
-let gcm_update_blocks_padded  ctx len text = gcm_update_blocks ctx len text
-
-
-inline_for_extraction
-val gcm_update_last:
-    ctx: gcm_ctx
-  -> len: size_t{v len < 16}
-  -> text: lbuffer uint8 len ->
-  Stack unit
-  (requires (fun h -> live h ctx /\ live h text))
-  (ensures (fun h0 _ h1 -> modifies1 ctx h0 h1))
-
-let gcm_update_last  ctx len text = poly #F32 ctx len text
+let gcm_update_blocks_padded ctx len text =
+  gcm_update_blocks ctx len text
 
 
-inline_for_extraction
+[@CInline]
 val gcm_emit:
-    tag: lbuffer uint8 16ul
-  -> ctx: gcm_ctx ->
+    tag:lbuffer uint8 16ul
+  -> ctx:gcm_ctx ->
   Stack unit
-  (requires (fun h -> live h ctx /\ live h tag))
-  (ensures (fun h0 _ h1 -> modifies1 tag h0 h1))
+  (requires fun h -> live h ctx /\ live h tag)
+  (ensures  fun h0 _ h1 -> modifies1 tag h0 h1)
 
 let gcm_emit tag ctx =
   let acc = get_acc ctx in
   decode tag acc
 
 
+[@CInline]
 val ghash:
-  tag: block
-  -> len: size_t
-  -> text: lbuffer uint8 len
-  -> key: block ->
+    tag:block
+  -> len:size_t
+  -> text:lbuffer uint8 len
+  -> key:block ->
   Stack unit
-  (requires (fun h -> live h tag /\ live h text /\ live h key))
-  (ensures (fun h0 _ h1 -> modifies1 tag h0 h1))
+  (requires fun h -> live h tag /\ live h text /\ live h key)
+  (ensures  fun h0 _ h1 -> modifies1 tag h0 h1)
 
 let ghash tag len text key =
-  ghash_mul_add #F32 tag len text key
+  ghash #Vec.PreComp tag len text key
