code/experimental/gf128/Hacl.Impl.Gf128.FieldNI.fst
@@ -2,16 +2,30 @@ module Hacl.Impl.Gf128.FieldNI
 
 open FStar.HyperStack
 open FStar.HyperStack.All
+open FStar.Mul
+
 open Lib.IntTypes
 open Lib.Buffer
 open Lib.IntVector
 
 module ST = FStar.HyperStack.ST
+module LSeq = Lib.Sequence
+module BSeq = Lib.ByteSequence
+
+module S = Spec.GF128
+module GF = Spec.GaloisField
+module Vec = Hacl.Spec.GF128.Vec
+
+
+#set-options "--z3rlimit 50 --max_fuel 1 --max_ifuel 1"
 
 inline_for_extraction noextract
 let vec128 = vec_t U128 1
 inline_for_extraction noextract
 let vec128_zero = vec_zero U128 1
+noextract
+let zero = GF.zero #S.gf128
+
 
 inline_for_extraction
 let cl_add (x:vec128) (y:vec128) : Tot vec128 = vec_xor x y
@@ -28,7 +42,6 @@ let clmul_wide (x:vec128) (y:vec128) : Tot (vec128 & vec128) =
   let lo = cl_add lo m2 in
   let hi = cl_add hi m1 in
   (hi,lo)
-
 
 inline_for_extraction
 let clmul_wide4
@@ -160,232 +173,262 @@ let gf128_reduce (hi:vec128) (lo:vec128) : Tot vec128 =
 let felem = lbuffer vec128 1ul
 let felem4 = lbuffer vec128 4ul
 let precomp = lbuffer vec128 4ul
+
 let block = lbuffer uint8 16ul
 let block4 = lbuffer uint8 64ul
-let gcm_ctx = lbuffer vec128 5ul // acc + precomp
+
+unfold noextract
+let op_String_Access #a #len = LSeq.index #a #len
 
 
-inline_for_extraction
-val get_acc: ctx:gcm_ctx ->
-  Stack felem
-  (requires (fun h -> live h ctx))
-  (ensures (fun h0 f h1 -> h0 == h1 /\ live h1 f /\ f == gsub ctx 0ul 1ul))
-
-let get_acc (ctx:gcm_ctx) =
-  sub ctx (size 0) (size 1)
+noextract
+let feval (h:mem) (f:felem) : GTot Vec.elem =
+  let f = as_seq h f in
+  (vec_v f.[0]).[0]
 
 
-inline_for_extraction
-val get_r: ctx:gcm_ctx ->
-  Stack felem
-  (requires (fun h -> live h ctx))
-  (ensures (fun h0 f h1 -> h0 == h1 /\ live h1 f /\ f == gsub ctx 4ul 1ul))
-
-let get_r (ctx:gcm_ctx) =
-  sub ctx (size 4) (size 1)
-
-
-inline_for_extraction
-val get_precomp: ctx: gcm_ctx ->
-  Stack precomp
-  (requires (fun h -> live h ctx))
-  (ensures (fun h0 f h1 -> h0 == h1 /\ live h1 f /\  f == gsub ctx 1ul 4ul))
-
-let get_precomp (ctx:gcm_ctx) =
-  sub ctx (size 1) (size 4)
+noextract
+let feval4 (h:mem) (f:felem4) : GTot Vec.elem4 =
+  let f = as_seq h f in
+  let f0 = (vec_v f.[0]).[0] in
+  let f1 = (vec_v f.[1]).[0] in
+  let f2 = (vec_v f.[2]).[0] in
+  let f3 = (vec_v f.[3]).[0] in
+  create4 f0 f1 f2 f3
 
 
 inline_for_extraction
 val create_felem: unit ->
   StackInline felem
-  (requires (fun h -> True))
-  (ensures (fun h0 f h1 -> live h1 f))
+  (requires fun h -> True)
+  (ensures  fun h0 f h1 ->
+    stack_allocated f h0 h1 (LSeq.create 1 vec128_zero) /\
+    feval h1 f == zero)
 
 let create_felem () = create 1ul vec128_zero
 
 
 inline_for_extraction
+val copy_felem: f1:felem -> f2:felem ->
+  Stack unit
+  (requires fun h -> live h f1 /\ live h f2 /\ disjoint f1 f2)
+  (ensures  fun h0 _ h1 -> modifies1 f1 h0 h1 /\
+    as_seq h1 f1 == as_seq h0 f2)
+
+let copy_felem f1 f2 =
+  let h0 = ST.get () in
+  f1.(0ul) <- f2.(0ul);
+  let h1 = ST.get () in
+  LSeq.eq_intro (as_seq h1 f1) (as_seq h0 f2)
+
+
+inline_for_extraction
 val felem_set_zero: f:felem ->
   Stack unit
-  (requires (fun h -> live h f))
-  (ensures (fun h0 _ h1 -> modifies1 f h0 h1))
+  (requires fun h -> live h f)
+  (ensures  fun h0 _ h1 -> modifies1 f h0 h1 /\
+    feval h1 f == zero)
 
-let felem_set_zero f =  f.(0ul) <- vec128_zero
+let felem_set_zero f = f.(0ul) <- vec128_zero
 
 
 inline_for_extraction
 val create_felem4: unit ->
   StackInline felem4
-  (requires (fun h -> True))
-  (ensures (fun h0 f h1 -> live h1 f))
+  (requires fun h -> True)
+  (ensures  fun h0 f h1 ->
+    stack_allocated f h0 h1 (LSeq.create 4 vec128_zero) /\
+    feval4 h1 f == LSeq.create 4 zero)
 
-let create_felem4 () = create 4ul vec128_zero
-
-
-inline_for_extraction
-val create_ctx: unit ->
-  StackInline gcm_ctx
-  (requires (fun h -> True))
-  (ensures (fun h0 f h1 -> live h1 f))
-
-let create_ctx () = create 5ul vec128_zero
+let create_felem4 () =
+  let f = create 4ul vec128_zero in
+  let h1 = ST.get () in
+  LSeq.eq_intro (feval4 h1 f) (LSeq.create 4 (u128 0));
+  f
 
 
 inline_for_extraction
 val load_felem:
-    x: felem
-  -> y: lbuffer uint8 16ul ->
+    x:felem
+  -> y:lbuffer uint8 16ul ->
   Stack unit
-  (requires (fun h -> live h x /\ live h y))
-  (ensures (fun h0 _ h1 -> modifies1 x h0 h1))
+  (requires fun h -> live h x /\ live h y)
+  (ensures  fun h0 _ h1 -> modifies1 x h0 h1 /\
+    feval h1 x == S.encode (as_seq h0 y))
 
 let load_felem x y =
-  x.(size 0) <- vec_load_be U128 1 y
+  let h0 = ST.get () in
+  x.(size 0) <- vec_load_be U128 1 y;
+  BSeq.index_uints_from_bytes_be #U128 #SEC #1 (as_seq h0 y) 0
 
 
 inline_for_extraction
 val load_felem4:
-    x: felem4
-  -> y: lbuffer uint8 64ul ->
+    x:felem4
+  -> y:block4 ->
   Stack unit
-  (requires (fun h -> live h x /\ live h y))
-  (ensures (fun h0 _ h1 -> modifies1 x h0 h1))
+  (requires fun h -> live h x /\ live h y /\ disjoint x y)
+  (ensures fun h0 _ h1 -> modifies1 x h0 h1 /\
+    feval4 h1 x == Vec.encode4 (as_seq h0 y))
 
 let load_felem4 x y =
+  let h0 = ST.get () in
   x.(size 0) <- vec_load_be U128 1 (sub y (size 0) (size 16));
+  BSeq.index_uints_from_bytes_be #U128 #SEC #1 (LSeq.sub (as_seq h0 y) 0 16) 0;
   x.(size 1) <- vec_load_be U128 1 (sub y (size 16) (size 16));
+  BSeq.index_uints_from_bytes_be #U128 #SEC #1 (LSeq.sub (as_seq h0 y) 16 16) 0;
   x.(size 2) <- vec_load_be U128 1 (sub y (size 32) (size 16));
-  x.(size 3) <- vec_load_be U128 1 (sub y (size 48) (size 16))
+  BSeq.index_uints_from_bytes_be #U128 #SEC #1 (LSeq.sub (as_seq h0 y) 32 16) 0;
+  x.(size 3) <- vec_load_be U128 1 (sub y (size 48) (size 16));
+  BSeq.index_uints_from_bytes_be #U128 #SEC #1 (LSeq.sub (as_seq h0 y) 48 16) 0
 
 
 inline_for_extraction
 val store_felem:
-    x: lbuffer uint8 16ul
-  -> y: felem ->
+    x:lbuffer uint8 16ul
+  -> y:felem ->
   Stack unit
-  (requires (fun h -> live h x /\ live h y))
-  (ensures (fun h0 _ h1 -> modifies1 x h0 h1))
+  (requires fun h -> live h x /\ live h y)
+  (ensures  fun h0 _ h1 -> modifies1 x h0 h1 /\
+    as_seq h1 x == S.store_elem (feval h0 y))
 
 let store_felem x y =
-  vec_store_be x y.(size 0)
+  let h0 = ST.get () in
+  vec_store_be x y.(size 0);
+  let h1 = ST.get () in
+  assert (as_seq h1 x == BSeq.uints_to_bytes_be (vec_v (as_seq h0 y).[0]));
+  //BSeq.index_uints_to_bytes_be #U128 #SEC #1 (vec_v (as_seq h0 y).[0]) 0;
+  //assert (LSeq.index (BSeq.uints_to_bytes_be (vec_v (as_seq h0 y).[0])) 0 == BSeq.uint_to_bytes_be (vec_v (as_seq h0 y).[0]).[0]);
+  //assert (BSeq.uints_to_bytes_be (vec_v (as_seq h0 y).[0]) == BSeq.uint_to_bytes_be (vec_v (as_seq h0 y).[0]).[0]);
+  admit()
 
 
-[@ CInline]
+[@CInline]
 val fadd:
     x: felem
   -> y: felem ->
   Stack unit
-  (requires (fun h -> live h x /\ live h y))
-  (ensures (fun h0 _ h1 -> modifies1 x h0 h1))
+  (requires fun h -> live h x /\ live h y)
+  (ensures  fun h0 _ h1 -> modifies1 x h0 h1 /\
+    feval h1 x == GF.fadd #S.gf128 (feval h0 x) (feval h0 y))
 
-let fadd (x:felem) (y:felem) =
+let fadd x y =
   x.(size 0) <- cl_add x.(size 0) y.(size 0)
+
+
+[@CInline]
+val fadd4:
+    x:felem4
+  -> y:felem4 ->
+  Stack unit
+  (requires fun h -> live h x /\ live h y)
+  (ensures  fun h0 _ h1 -> modifies1 x h0 h1 /\
+    feval4 h1 x == Vec.fadd4 (feval4 h0 x) (feval4 h0 y))
+
+let fadd4 x y =
+  let (x0, x1, x2, x3) = (x.(0ul), x.(1ul), x.(2ul), x.(3ul)) in
+  let (y0, y1, y2, y3) = (y.(0ul), y.(1ul), y.(2ul), y.(3ul)) in
+  let h0 = ST.get () in
+  x.(size 0) <- cl_add x0 y0;
+  x.(size 1) <- cl_add x1 y1;
+  x.(size 2) <- cl_add x2 y2;
+  x.(size 3) <- cl_add x3 y3;
+  let h1 = ST.get () in
+  LSeq.eq_intro (feval4 h1 x) (Vec.fadd4 (feval4 h0 x) (feval4 h0 y))
 
 
 [@ CInline]
 val fmul:
-    x: felem
-  -> y: felem ->
+    x:felem
+  -> y:felem ->
   Stack unit
-  (requires (fun h -> live h x /\ live h y))
-  (ensures (fun h0 _ h1 -> modifies1 x h0 h1))
+  (requires fun h -> live h x /\ live h y)
+  (ensures  fun h0 _ h1 -> modifies1 x h0 h1 /\
+    feval h1 x == GF.fmul_be #S.gf128 (feval h0 x) (feval h0 y))
 
-let fmul (x:felem) (y:felem) =
+let fmul x y =
   let xe = x.(size 0) in
   let ye = y.(size 0) in
   let (hi,lo) = clmul_wide xe ye in
   let lo = gf128_reduce hi lo in
-  x.(size 0) <- lo
+  let h0 = ST.get () in
+  x.(size 0) <- lo;
+  let h1 = ST.get () in
+  assume (feval h1 x == GF.fmul_be #S.gf128 (feval h0 x) (feval h0 y))
 
 
-[@ CInline]
+[@CInline]
 val load_precompute_r:
-    pre: precomp
-  -> key: block ->
+    pre:precomp
+  -> key:block ->
   Stack unit
-  (requires (fun h -> live h pre /\ live h key))
-  (ensures (fun h0 _ h1 -> modifies1 pre h0 h1))
+  (requires fun h -> live h pre /\ live h key /\ disjoint pre key)
+  (ensures  fun h0 _ h1 -> modifies1 pre h0 h1 /\
+    (let r = S.load_elem (as_seq h0 key) in
+    feval4 h1 pre == Vec.load_precompute_r r))
 
 let load_precompute_r pre key =
-  let r_4 = sub pre (size 0) (size 1) in
-  let r_3 = sub pre (size 1) (size 1) in
-  let r_2 = sub pre (size 2) (size 1) in
-  let r   = sub pre (size 3) (size 1) in
-  load_felem r key;
-  pre.(size 0) <- r.(size 0);
-  pre.(size 1) <- r.(size 0);
-  pre.(size 2) <- r.(size 0);
-  fmul r_2 r;
-  fmul r_3 r_2;
-  fmul r_4 r_3
+  let r4 = sub pre (size 0) (size 1) in
+  let r3 = sub pre (size 1) (size 1) in
+  let r2 = sub pre (size 2) (size 1) in
+  let r1 = sub pre (size 3) (size 1) in
+
+  load_felem r1 key;
+  copy_felem r4 r1;
+  copy_felem r3 r1;
+  copy_felem r2 r1;
+  fmul r2 r1;
+  fmul r3 r2;
+  fmul r4 r3
 
 
-[@ CInline]
+[@CInline]
 val fmul_pre:
-    x: felem
-  -> y: precomp ->
+    x:felem
+  -> y:precomp ->
   Stack unit
-  (requires (fun h -> live h x /\ live h y))
-  (ensures (fun h0 _ h1 -> modifies1 x h0 h1))
+  (requires fun h -> live h x /\ live h y)
+  (ensures  fun h0 _ h1 -> modifies1 x h0 h1 /\
+    feval h1 x == GF.fmul_be #S.gf128 (feval h0 x) (feval h0 (gsub y 0ul 1ul)))
 
 let fmul_pre x pre =
-  let r = sub pre (size 3) (size 1) in
-  let xe = x.(size 0) in
-  let ye = r.(size 0) in
-  let (hi,lo) = clmul_wide xe ye in
-  let lo = gf128_reduce hi lo in
-  x.(size 0) <- lo
+  let r = sub pre (size 0) (size 1) in
+  fmul x r
 
 
-[@ CInline]
-val fadd4:
-    x: felem4
-  -> y: felem4 ->
+[@CInline]
+val fmul_r4:
+    x:felem4
+  -> pre:precomp ->
   Stack unit
-  (requires (fun h -> live h x /\ live h y))
-  (ensures (fun h0 _ h1 -> modifies1 x h0 h1))
+  (requires fun h -> live h x /\ live h pre /\ disjoint x pre)
+  (ensures  fun h0 _ h1 -> modifies1 x h0 h1 /\
+    (let r4 = feval h0 (gsub pre 0ul 1ul) in
+    feval4 h1 x == Vec.fmul4 (feval4 h0 x) (create4 r4 r4 r4 r4)))
 
-let fadd4 (x:felem4) (y:felem4) =
-  let x0 = x.(0ul) in
-  let x1 = x.(1ul) in
-  let x2 = x.(2ul) in
-  let x3 = x.(3ul) in
-  let y0 = y.(0ul) in
-  let y1 = y.(1ul) in
-  let y2 = y.(2ul) in
-  let y3 = y.(3ul) in
-
-  x.(size 0) <- cl_add x0 y0;
-  x.(size 1) <- cl_add x1 y1;
-  x.(size 2) <- cl_add x2 y2;
-  x.(size 2) <- cl_add x3 y3
-
-
-[@ CInline]
-val fmul4:
-    x: felem4
-  -> pre: precomp ->
-  Stack unit
-  (requires (fun h -> live h x /\ live h pre))
-  (ensures (fun h0 _ h1 -> modifies1 x h0 h1))
-
-let fmul4 (x:felem4) (pre:precomp) =
+let fmul_r4 x pre =
+  let h0 = ST.get () in
   fmul (sub x (size 0) (size 1)) (sub pre (size 0) (size 1));
   fmul (sub x (size 1) (size 1)) (sub pre (size 0) (size 1));
   fmul (sub x (size 2) (size 1)) (sub pre (size 0) (size 1));
-  fmul (sub x (size 3) (size 1)) (sub pre (size 0) (size 1))
+  fmul (sub x (size 3) (size 1)) (sub pre (size 0) (size 1));
+  let h1 = ST.get () in
+  let r4 = feval h0 (gsub pre 0ul 1ul) in
+  LSeq.eq_intro (feval4 h1 x) (Vec.fmul4 (feval4 h0 x) (create4 r4 r4 r4 r4))
 
 
-[@ CInline]
-val fadd_mul4:
-    acc: felem
-  -> x: felem4
-  -> pre: precomp ->
+[@CInline]
+val normalize4:
+    acc:felem
+  -> x:felem4
+  -> pre:precomp ->
   Stack unit
-  (requires (fun h -> live h acc /\ live h x /\ live h pre))
-  (ensures (fun h0 _ h1 -> modifies1 acc h0 h1))
+  (requires fun h -> live h acc /\ live h x /\ live h pre)
+  (ensures  fun h0 _ h1 -> modifies1 acc h0 h1 /\
+   (let x = Vec.fadd4 (create4 (feval h0 acc) GF.zero GF.zero GF.zero) (feval4 h0 x) in
+    feval h1 acc == Vec.normalize4 x (feval4 h0 pre)))
 
-let fadd_mul4 (acc:felem) (x:felem4) (pre:precomp) =
+let normalize4 acc x pre =
   let x1 = x.(size 0) in
   let x2 = x.(size 1) in
   let x3 = x.(size 2) in
@@ -395,7 +438,13 @@ let fadd_mul4 (acc:felem) (x:felem4) (pre:precomp) =
   let y3 = pre.(size 2) in
   let y4 = pre.(size 3) in
   let acc0 = acc.(size 0) in
+
   let acc0 = cl_add acc0 x1 in
   let (hi,lo) = clmul_wide4 acc0 x2 x3 x4 y1 y2 y3 y4 in
   let lo = gf128_reduce hi lo in
-  acc.(size 0) <- lo
+  let h0 = ST.get () in
+  acc.(size 0) <- lo;
+  let h1 = ST.get () in
+  assume (
+    let x = Vec.fadd4 (create4 (feval h0 acc) GF.zero GF.zero GF.zero) (feval4 h0 x) in
+    feval h1 acc == Vec.normalize4 x (feval4 h0 pre))
