code/experimental/gf128/Hacl.Impl.Gf128.Generic.fst
@@ -2,315 +2,307 @@ module Hacl.Impl.Gf128.Generic
 
 open FStar.HyperStack
 open FStar.HyperStack.All
+
 open Lib.IntTypes
 open Lib.Buffer
+
 open Hacl.Impl.Gf128.Fields
 
 module ST = FStar.HyperStack.ST
+module LSeq = Lib.Sequence
+
+module S = Spec.GF128
+module GF = Spec.GaloisField
+module Vec = Hacl.Spec.GF128.Vec
 
 
 #set-options "--z3rlimit 50 --max_fuel 0"
 
+inline_for_extraction noextract
+let gcm_ctx (s:field_spec) = lbuffer (elem_t s) (felem_len s +! precomp_len s)
+
+inline_for_extraction noextract
+let get_acc #s (ctx:gcm_ctx s) = sub ctx 0ul (felem_len s)
+
+inline_for_extraction noextract
+let get_r #s (ctx:gcm_ctx s) = sub ctx (felem4_len s) (felem_len s)
+
+inline_for_extraction noextract
+let get_precomp #s (ctx:gcm_ctx s) = sub ctx (felem_len s) (precomp_len s)
+
+
 inline_for_extraction
 val encode:
-    #s: field_spec
-  -> x: felem s
+    #s:field_spec
+  -> x:felem s
   -> y:block ->
   Stack unit
-  (requires (fun h -> live h x /\ live h y))
-  (ensures (fun h0 _ h1 -> modifies1 x h0 h1))
+  (requires fun h -> live h x /\ live h y)
+  (ensures  fun h0 _ h1 -> modifies1 x h0 h1 /\
+    feval h1 x == S.encode (as_seq h0 y))
 
 let encode #s x y = load_felem x y
 
 
 inline_for_extraction
 val encode4:
-    #s: field_spec
-  -> x: felem4 s
-  -> y: block4 ->
+    #s:field_spec
+  -> x:felem4 s
+  -> y:block4 ->
   Stack unit
-  (requires (fun h -> live h x /\ live h y))
-  (ensures (fun h0 _ h1 -> modifies1 x h0 h1))
+  (requires fun h -> live h x /\ live h y /\ disjoint x y)
+  (ensures  fun h0 _ h1 -> modifies1 x h0 h1 /\
+    feval4 h1 x == Vec.encode4 (as_seq h0 y))
 
 let encode4 #s x y = load_felem4 x y
 
 
 inline_for_extraction
 val decode:
-    #s: field_spec
-  -> y: block
-  -> x: felem s ->
+    #s:field_spec
+  -> x:block
+  -> y:felem s ->
   Stack unit
-  (requires (fun h -> live h x /\ live h y))
-  (ensures (fun h0 _ h1 -> modifies1 y h0 h1))
+  (requires fun h -> live h x /\ live h y)
+  (ensures  fun h0 _ h1 -> modifies1 x h0 h1 /\
+    as_seq h1 x == S.decode (feval #s h0 y))
 
-let decode #s y x = store_felem y x
+let decode #s x y = store_felem x y
 
 
 inline_for_extraction
 val encode_last:
-    #s: field_spec
-  -> x: felem s
-  -> len: size_t{v len < 16}
-  -> y: lbuffer uint8 len ->
+    #s:field_spec
+  -> x:felem s
+  -> len:size_t{v len < 16}
+  -> y:lbuffer uint8 len ->
   Stack unit
-  (requires (fun h -> live h x /\ live h y))
-  (ensures (fun h0 _ h1 -> modifies1 x h0 h1))
+  (requires fun h -> live h x /\ live h y)
+  (ensures  fun h0 _ h1 -> modifies1 x h0 h1 /\
+    feval h1 x == S.encode_last (v len) (as_seq h0 y))
 
 let encode_last #s x len y =
   push_frame();
   let b = create 16ul (u8 0) in
-  copy (sub b 0ul len) y;
+  update_sub b 0ul len y;
   encode x b;
   pop_frame()
 
 
 inline_for_extraction
-val update:
-    #s: field_spec
-  -> acc: felem s
-  -> x: block
-  -> r: felem s ->
+val gf128_update1:
+    #s:field_spec
+  -> acc:felem s
+  -> x:block
+  -> r:felem s ->
   Stack unit
-  (requires (fun h -> live h x /\ live h r /\ live h acc))
-  (ensures (fun h0 _ h1 -> modifies1 acc h0 h1))
+  (requires fun h -> live h x /\ live h r /\ live h acc)
+  (ensures  fun h0 _ h1 -> modifies1 acc h0 h1 /\
+    feval h1 acc == S.gf128_update1 (feval h0 r) (as_seq h0 x) (feval h0 acc))
 
-inline_for_extraction
-let update #s acc x r =
+let gf128_update1 #s acc x r =
   push_frame();
   let elem = create_felem s in
   encode elem x;
   fadd acc elem;
   fmul acc r;
-  pop_frame()
+  pop_frame(); admit()
 
+(*
+let gf128_update1 (r:elem) (b:lbytes size_block) (acc:elem) : Tot elem =
+(encode b `fadd` acc) `fmul_be` r
+*)
 
 inline_for_extraction
-val update_last:
-    #s: field_spec
-  -> acc: felem s
-  -> len: size_t{v len < 16}
-  -> x: lbuffer uint8 len
-  -> r: felem s ->
+val gf128_update_last:
+    #s:field_spec
+  -> acc:felem s
+  -> len:size_t{v len < 16}
+  -> x:lbuffer uint8 len
+  -> r:felem s ->
   Stack unit
-  (requires (fun h -> live h x /\ live h r /\ live h acc))
-  (ensures (fun h0 _ h1 -> modifies1 acc h0 h1))
+  (requires fun h -> live h x /\ live h r /\ live h acc)
+  (ensures  fun h0 _ h1 -> modifies1 acc h0 h1 /\
+    feval h1 acc == S.gf128_update_last (feval h0 r) (v len) (as_seq h0 x) (feval h0 acc))
 
-inline_for_extraction
-let update_last #s acc l x r =
+let gf128_update_last #s acc l x r =
   push_frame();
   let elem = create_felem s in
   encode_last elem l x;
   fadd acc elem;
   fmul acc r;
-  pop_frame()
+  pop_frame(); admit()
 
+(*
+let gf128_update_last (r:elem) (l:size_nat{l < size_block}) (b:lbytes l) (acc:elem) =
+  if l = 0 then acc else (encode_last l b `fadd` acc) `fmul_be` r
+*)
 
 inline_for_extraction
-val poly:
-    #s: field_spec
-  -> ctx: gcm_ctx s
-  -> len: size_t
-  -> text: lbuffer uint8 len ->
+val gf128_update_scalar:
+    #s:field_spec
+  -> acc:felem s
+  -> r:felem s
+  -> len:size_t
+  -> text:lbuffer uint8 len ->
   Stack unit
-  (requires (fun h -> live h ctx /\ live h text))
-  (ensures (fun h0 _ h1 -> modifies1 ctx h0 h1))
+  (requires fun h -> live h acc /\ live h r /\ live h text)
+  (ensures  fun h0 _ h1 -> modifies1 acc h0 h1 /\
+    feval h1 acc == S.gf128_update (as_seq h0 text) (feval h0 acc) (feval h0 r))
 
-let poly #s ctx len text =
-  let acc = get_acc ctx in
-  let r = get_r ctx in
+let gf128_update_scalar #s acc r len text =
   let blocks = len /. size 16 in
   let h2 = ST.get() in
-  loop_nospec #h2 blocks acc (fun i ->
-    let tb = (sub text (i *. size 16) (size 16)) in
-    update #s acc tb r);
-  let rem = len %. size 16 in
-  if (rem >. size 0) then (
-    let last = sub text (blocks *. size 16) rem in
-    update_last #s acc rem last r)
 
-
-inline_for_extraction
-val poly_pre:
-    #s: field_spec
-  -> ctx: gcm_ctx s
-  -> len: size_t
-  -> text: lbuffer uint8 len ->
-  Stack unit
-  (requires (fun h -> live h ctx /\ live h text))
-  (ensures (fun h0 _ h1 -> modifies1 ctx h0 h1))
-
-let poly_pre #s ctx len text =
-  push_frame ();
-  let acc = get_acc ctx in
-  let pre = get_precomp ctx in
-  let b = create_felem s in
-  let blocks = len /. size 16 in
-  let h0 = ST.get() in
-  loop_nospec2 #h0 blocks acc b (fun i ->
+  loop_nospec #h2 blocks acc
+  (fun i ->
     let tb = sub text (i *. size 16) (size 16) in
-    encode b tb;
-    fadd acc b;
-    fmul_pre acc pre);
+    gf128_update1 #s acc tb r);
+
   let rem = len %. size 16 in
   if (rem >. size 0) then (
     let last = sub text (blocks *. size 16) rem in
-    encode_last b rem last;
-    fadd acc b;
-    fmul_pre acc pre);
-  pop_frame()
+    gf128_update_last #s acc rem last r); admit()
 
-
+//NI
 inline_for_extraction
-val poly4_add_mul:
-    #s: field_spec
-  -> ctx: gcm_ctx s
-  -> len: size_t
-  -> text: lbuffer uint8 len ->
+val gf128_update_multi_add_mul:
+    #s:field_spec
+  -> acc:felem s
+  -> pre:precomp s
+  -> len:size_t{0 < v len /\ v len % 64 = 0}
+  -> text:lbuffer uint8 len ->
   Stack unit
-  (requires (fun h -> live h ctx /\ live h text))
-  (ensures (fun h0 _ h1 -> modifies1 ctx h0 h1))
+  (requires fun h -> live h acc /\ live h pre /\ live h text)
+  (ensures  fun h0 _ h1 -> modifies1 acc h0 h1 /\
+    feval h1 acc == Vec.gf128_update_multi_add_mul (as_seq h0 text) (feval h0 acc) (get_r1 h0 pre))
 
-let poly4_add_mul #s ctx len text =
+let gf128_update_multi_add_mul #s acc pre len text =
   push_frame ();
-  let acc = get_acc ctx in
-  let pre = get_precomp ctx in
   let b4 = create_felem4 s in
   let blocks = len /. size 64 in
+
   let h0 = ST.get() in
   loop_nospec2 #h0 blocks acc b4
-    (fun i -> let tb = sub text (i *. size 64) (size 64) in
-           encode4 b4 tb;
-           fadd_mul4 acc b4 pre );
-  let rem = len %. size 64 in
-  let last = sub text (blocks *. size 64) rem in
-  poly #s ctx rem last;
-  pop_frame()
+  (fun i ->
+    let tb = sub text (i *. size 64) (size 64) in
+    encode4 b4 tb;
+    normalize4 acc b4 pre);
+  pop_frame (); admit()
 
-
-#set-options "--z3rlimit 1000 --max_fuel 1"
-
+//PreComp
 inline_for_extraction
-val poly4_mul_add:
-    #s: field_spec
-  -> ctx: gcm_ctx s
-  -> len: size_t
-  -> text: lbuffer uint8 len ->
+val gf128_update_multi_mul_add:
+    #s:field_spec
+  -> acc:felem s
+  -> pre:precomp s
+  -> len:size_t{0 < v len /\ v len % 64 = 0}
+  -> text:lbuffer uint8 len ->
   Stack unit
-  (requires (fun h -> live h ctx /\ live h text /\ s == F32))
-  (ensures (fun h0 _ h1 -> modifies1 ctx h0 h1))
+  (requires fun h -> live h acc /\ live h pre /\ live h text)
+  (ensures  fun h0 _ h1 -> modifies1 acc h0 h1 /\
+    feval h1 acc == Vec.gf128_update_multi_mul_add (as_seq h0 text) (feval h0 acc) (get_r1 h0 pre))
 
-let poly4_mul_add #s ctx len text =
-  let h0 = ST.get () in
+let gf128_update_multi_mul_add #s acc pre len text =
   push_frame ();
-  let h1 = ST.get () in
   let b4 = create_felem4 s in
   let acc4 = create_felem4 s in
-  let h2 = ST.get () in
-  let acc = get_acc ctx in
-  let pre = get_precomp ctx in
-  copy (sub acc4 0ul (felem_len s)) acc;
-  let h3 = ST.get () in
-  assert(modifies1 acc4 h2 h3);
-  let blocks = len /. size 64 in
-  if (blocks >. 0ul) then (
-    let h4 = ST.get () in
-    let tb = sub text (size 0) (size 64) in
+  copy_felem (sub acc4 0ul (felem_len s)) acc;
+
+  let tb = sub text 0ul 64ul in
+  encode4 b4 tb;
+  fadd4 acc4 b4;
+
+  let len1 = len -! 64ul in
+  let blocks = len1 /. 64ul in
+  let text1 = sub text 64ul len1 in
+  let h0 = ST.get () in
+  loop_nospec2 #h0 blocks b4 acc4
+  (fun i ->
+    let tb = sub text1 (i *. 64ul) 64ul in
     encode4 b4 tb;
-    fadd4 acc4 b4;
-    let h5 = ST.get() in
-    loop_nospec2 #h5 (blocks -. 1ul) b4 acc4 (fun i ->
-      let tb = sub text ((i +. size 1) *. size 64) (size 64) in
-      encode4 b4 tb;
-      fmul4 acc4 pre;
-      fadd4 acc4 b4);
-    let r4 = sub pre 0ul 2ul in
-    let r3 = sub pre 2ul 2ul in
-    let r2 = sub pre 4ul 2ul in
-    let r = sub pre 6ul 2ul in
-    let acc0 = sub acc4 0ul 2ul in
-    let acc1 = sub acc4 2ul 2ul in
-    let acc2 = sub acc4 4ul 2ul in
-    let acc3 = sub acc4 6ul 2ul in
-    fmul acc0 r4;
-    fmul acc1 r3;
-    fmul acc2 r2;
-    fmul acc3 r;
-    copy acc acc0;
-    fadd acc acc1;
-    fadd acc acc2;
-    fadd acc acc3;
-    let h10 = ST.get() in
-    assert(modifies3 acc b4 acc4 h3 h10)
-  )
-  else (
-    let h11 = ST.get () in
-    modifies1_is_modifies3 acc b4 acc4 h3 h11
-  );
-  let rem = len %. size 64 in
-  let last = sub text (blocks *. size 64) rem in
-  poly #s ctx rem last;
-  let h13 = ST.get () in
-  assert(modifies3 ctx b4 acc4 h2 h13);
-  pop_frame();
-  let h14 = ST.get () in
-  assert(modifies1 ctx h0 h14)
+    fmul_r4 acc4 pre;
+    fadd4 acc4 b4);
+  felem_set_zero acc;
+  normalize4 acc acc4 pre;
+  pop_frame (); admit()
+
+
+inline_for_extraction
+val gf128_update_multi:
+    #s:field_spec
+  -> acc:felem s
+  -> pre:precomp s
+  -> len:size_t{0 < v len /\ v len % 64 = 0}
+  -> text:lbuffer uint8 len ->
+  Stack unit
+  (requires fun h -> live h acc /\ live h pre /\ live h text)
+  (ensures  fun h0 _ h1 -> modifies1 acc h0 h1 /\
+    feval h1 acc == Vec.gf128_update_multi s (as_seq h0 text) (feval h0 acc) (get_r1 h0 pre))
+
+let gf128_update_multi #s acc pre len text =
+  match s with
+  | Vec.NI -> gf128_update_multi_add_mul acc pre len text
+  | Vec.PreComp -> gf128_update_multi_mul_add acc pre len text
+
+
+inline_for_extraction
+val gf128_update_vec:
+    #s:field_spec
+  -> acc:felem s
+  -> pre:precomp s
+  -> len:size_t
+  -> text:lbuffer uint8 len ->
+  Stack unit
+  (requires fun h -> live h acc /\ live h pre /\ live h text)
+  (ensures  fun h0 _ h1 -> modifies1 acc h0 h1 /\
+    feval h1 acc == Vec.gf128_update_vec s (as_seq h0 text) (feval h0 acc) (get_r1 h0 pre))
+
+let gf128_update_vec #s acc pre len text =
+  let len0 = len /. 64ul *. 64ul in
+  let t0 = sub text 0ul len0 in
+  if (len0 >. 0ul) then gf128_update_multi #s acc pre len0 t0;
+
+  let len1 = len -! len0 in
+  let t1 = sub text len0 len1 in
+  let r1 = sub pre (3ul *. felem_len s) (felem_len s) in
+  gf128_update_scalar #s acc r1 len1 t1; admit()
 
 
 inline_for_extraction
 val gcm_init:
-    #s: field_spec
-  -> ctx: gcm_ctx s
-  -> key: block ->
+    #s:field_spec
+  -> ctx:gcm_ctx s
+  -> key:block ->
   Stack unit
-  (requires (fun h -> live h ctx /\ live h key))
-  (ensures (fun h0 _ h1 -> modifies1 ctx h0 h1))
+  (requires fun h -> live h ctx /\ live h key /\ disjoint ctx key)
+  (ensures  fun h0 _ h1 -> modifies1 ctx h0 h1)
 
 let gcm_init #s ctx key =
   let acc = get_acc ctx in
   let pre = get_precomp ctx in
+
   felem_set_zero acc;
   load_precompute_r pre key
 
 
 inline_for_extraction
-val ghash_add_mul:
-    #s: field_spec
-  -> tag: block
-  -> len: size_t
-  -> text: lbuffer uint8 len
-  -> key: block ->
+val ghash:
+    #s:field_spec
+  -> tag:block
+  -> len:size_t
+  -> text:lbuffer uint8 len
+  -> key:block ->
   Stack unit
-  (requires (fun h -> live h tag /\ live h text /\ live h key))
-  (ensures (fun h0 _ h1 -> modifies1 tag h0 h1))
+  (requires fun h -> live h tag /\ live h text /\ live h key)
+  (ensures  fun h0 _ h1 -> modifies1 tag h0 h1)
 
-let ghash_add_mul #s tag len text key =
+let ghash #s tag len text key =
   push_frame();
-  let ctx = create_ctx s in
+  let ctx : gcm_ctx s = create (felem_len s +! precomp_len s) (elem_zero s) in
   gcm_init ctx key;
-  poly4_add_mul ctx len text;
   let acc = get_acc ctx in
-  decode tag acc;
-  pop_frame()
-
-
-inline_for_extraction
-val ghash_mul_add:
-    #s: field_spec
-  -> tag: block
-  -> len: size_t
-  -> text: lbuffer uint8 len
-  -> key: block ->
-  Stack unit
-  (requires (fun h -> s == F32 /\ live h tag /\ live h text /\ live h key))
-  (ensures (fun h0 _ h1 -> modifies1 tag h0 h1))
-
-let ghash_mul_add #s tag len text key =
-  push_frame();
-  let ctx = create_ctx s in
-  gcm_init ctx key;
-  poly4_mul_add ctx len text;
-//  poly_pre ctx len text;
-  let acc = get_acc ctx in
+  let pre = get_precomp ctx in
+  gf128_update_vec acc pre len text;
   decode tag acc;
   pop_frame()
